more

haskell/Optics2/src/Traversable.hs
@@ -1,0 +1,36 @@
+module  Traversable
+    (   Traversable     (..)
+    )   where
+
+-- Data.Traversable
+
+import Prelude hiding (Traversable, traverse, sequenceA)
+
+import Control.Applicative
+
+class (Functor t, Foldable t) => Traversable t where
+    {-# MINIMAL traverse | sequenceA #-}
+    
+    traverse :: Applicative f => (a -> f b) -> t a -> f (t b)
+    traverse f = sequenceA . fmap f
+
+    sequenceA :: Applicative f => t (f a) -> f (t a)
+    sequenceA = traverse id 
+
+    mapM :: Monad m => (a -> m b) -> t a -> m (t b)
+    mapM = traverse
+
+    sequence :: Monad m => t (m a) -> m (t a)
+    sequence = sequenceA
+
+instance Traversable Maybe where
+    traverse _ Nothing = pure Nothing
+    traverse f (Just x) = Just <$> f x 
+
+instance Traversable [] where
+    traverse _ [] = pure []
+    traverse f (x : xs) =  liftA2 (:) (f x) (traverse f xs)
+
+instance Traversable (Either a) where
+    traverse _ (Left x) = pure (Left x)
+    traverse f (Right y) = Right <$> f y
